@prefix rdf: <http://www.w3.org/1999/02/22-rdf-syntax-ns#> .
@prefix owl: <http://www.w3.org/2002/07/owl#> .
@prefix adms: <http://www.w3.org/ns/adms#> .
@prefix dcterms: <http://purl.org/dc/terms/> .
@prefix xsd: <http://www.w3.org/2001/XMLSchema#> .
@prefix vann: <http://purl.org/vocab/vann/> .
@prefix foaf: <http://xmlns.com/foaf/0.1/> .
@prefix dc: <http://purl.org/dc/elements/1.1/> .
@prefix pdo: <http://ontologies.smile.deri.ie/pdo#> .
@prefix rdfs: <http://www.w3.org/2000/01/rdf-schema#> .

<http://vocab.deri.ie/pdo> a owl:Ontology, adms:SemanticAsset;
    dcterms:title "Project Documents Ontology";
    dcterms:description "The Project Documents Ontology, described using W3C RDF Schema and the Web Ontology Language, models the inherent structure and concepts of various documents in a project-specific setting, like meeting minutes, status reports etc.";
    dcterms:modified "2010-07-09"^^xsd:date;
    vann:preferredNamespaceUri "http://ontologies.smile.deri.ie/pdo#";
    vann:preferredNamespacePrefix "pdo";
    foaf:homepage <http://vocab.deri.ie/pdo.html>;
    dcterms:created "2010-07-09"^^xsd:date;
    dcterms:publisher "http://vocab.deri.ie/pdo#DERI%2C%20NUI%20Galway";
    dcterms:partOf <http://vocab.deri.ie>;
    dcterms:type <http://purl.org/adms/assettype/Ontology>;
    dcterms:status <http://purl.org/adms/status/UnderDevelopment>;
    dc:creator <http://vocab.deri.ie/pdo#pravar> .

<http://vocab.deri.ie/pdo#ttl> a adms:SemanticDistribution;
    dcterms:FileFormat <>;
    adms:accessURL "http://vocab.deri.ie/pdo.ttl";
    adms:status <http://purl.org/adms/status/Completed> .

<http://vocab.deri.ie/pdo#rdf> a adms:SemanticDistribution;
    dcterms:FileFormat <>;
    adms:accessURL "http://vocab.deri.ie/pdo.rdf";
    adms:status <http://purl.org/adms/status/Completed> .

<http://vocab.deri.ie/pdo#pravar> a foaf:Person;
    foaf:name "Pradeep Varma";
    foaf:homepage <>;
    foaf:mbox <mailto:pradeep.varma@deri.org> .

<http://vocab.deri.ie/pdo#DERI%2C%20NUI%20Galway> a dcterms:Agent;
    foaf:member <http://vocab.deri.ie/pdo#pravar>;
    foaf:name "DERI, NUI Galway";
    foaf:homepage <http://deri.ie/> .

pdo:Absentee a rdfs:Class, owl:Class;
    rdfs:label "Absentee";
    rdfs:comment "Models the absentee role of a person in a meeting context.";
    rdfs:subClassOf pdo:PersonRole .

pdo:ActionItem a rdfs:Class, owl:Class;
    rdfs:label "ActionItem";
    rdfs:comment "Subclasses pdo:Artifact and models the structure of an action item/task";
    rdfs:subClassOf pdo:Artefact .

pdo:AgendaItem a rdfs:Class, owl:Class;
    rdfs:label "AgendaItem";
    rdfs:comment "Subclasses pdo:Artifact and models the structure of an agenda item";
    rdfs:subClassOf pdo:Artefact .

pdo:Artefact a rdfs:Class, owl:Class;
    rdfs:label "Artefact";
    rdfs:comment "An abstract class for  any kind of information artifact which can be structured according to its sematics." .

pdo:Attendee a rdfs:Class, owl:Class;
    rdfs:label "Attendee";
    rdfs:comment "Models the attendee role of a person in a meeting context.";
    rdfs:subClassOf pdo:PersonRole .

pdo:Chair a rdfs:Class, owl:Class;
    rdfs:label "Chair";
    rdfs:comment "Models the chair role of a person in a meeting context.";
    rdfs:subClassOf pdo:PersonRole .

pdo:Comment a rdfs:Class, owl:Class;
    rdfs:label "Comment";
    rdfs:comment "Models a comment made by a person" .

pdo:Document a rdfs:Class, owl:Class;
    rdfs:label "Document";
    rdfs:comment "The base class for all kinds of electronic documents in a project-specific setting.";
    rdfs:subClassOf foaf:Document .

pdo:LeaveReport a rdfs:Class, owl:Class;
    rdfs:label "LeaveReport";
    rdfs:comment "Subclasses pdo:Artefact and models the structure of a leave report";
    rdfs:subClassOf
        pdo:LeaveReport,
        pdo:Report .

pdo:Meeting a rdfs:Class, owl:Class;
    rdfs:label "Meeting";
    rdfs:comment "The class modelling the actual meeting which is the subject of a particular minutes document." .

pdo:MeetingMinutes a rdfs:Class, owl:Class;
    rdfs:label "Minutes";
    rdfs:comment "The class modelling the structure and cotent of an electronic version of the minutes of a meetintg.";
    rdfs:subClassOf pdo:Document .

pdo:PersonRole a rdfs:Class, owl:Class;
    rdfs:label "PersonRole";
    rdfs:comment "The abstract class modelling various roles taken by individuals during a particular context ( for example, the attendees, scribe etc in a meeting or the reporter in a status report.)" .

pdo:Poll a rdfs:Class, owl:Class;
    rdfs:label "Poll";
    rdfs:comment "Subclasses pdo:Artifact and models the structure of a poll";
    rdfs:subClassOf pdo:Artefact .

pdo:PollOption a rdfs:Class, owl:Class;
    rdfs:label "PollOption";
    rdfs:comment "Models an option in a poll. Each option is linked to a list of people who selected the option during the poll" .

pdo:Presenter a rdfs:Class, owl:Class;
    rdfs:label "Presenter";
    rdfs:comment "Models the presenter role of a person in the context of an agenda item.";
    rdfs:subClassOf pdo:PersonRole .

pdo:Publication a rdfs:Class, owl:Class;
    rdfs:label "Publication";
    rdfs:comment "Subclasses pdo:Artifact and uses bibliography ontology to model the structure of a publication";
    rdfs:subClassOf pdo:Artefact .

pdo:Report a rdfs:Class, owl:Class;
    rdfs:label "TravelReport";
    rdfs:comment "Subclasses pdo:Artefact and models the structure of a travel report";
    rdfs:subClassOf pdo:Artefact .

pdo:Reporter a rdfs:Class, owl:Class;
    rdfs:label "Reporter";
    rdfs:comment "Models the reporting role of a person in a status reporting context.";
    rdfs:subClassOf pdo:PersonRole .

pdo:Scribe a rdfs:Class, owl:Class;
    rdfs:label "Scribe";
    rdfs:comment "Models the scribe role of a person in a meeting context.";
    rdfs:subClassOf pdo:PersonRole .

pdo:StatusReport a rdfs:Class, owl:Class;
    rdfs:label "Report";
    rdfs:comment "The class modelling the structure and content of an electronic version of a status reports document";
    rdfs:subClassOf pdo:Document .

pdo:TravelReport a rdfs:Class, owl:Class;
    rdfs:label "TravelReport";
    rdfs:comment "Subclasses pdo:Artefact and models the structure of a travel report";
    rdfs:subClassOf pdo:Report .

pdo:hasAlias a rdf:Property, owl:DatatypeProperty;
    rdfs:label "hasAlias";
    rdfs:comment "A way to store different alias names of objects (used internally by the application)";
    rdfs:domain owl:Thing;
    rdfs:range xsd:string .

pdo:hasCreationTime a rdf:Property, owl:DatatypeProperty;
    rdfs:label "hasCreationTime";
    rdfs:domain pdo:ActionItem;
    rdfs:range xsd:dateTime .

pdo:hasDescription a rdf:Property, owl:DatatypeProperty;
    rdfs:label "hasDescription";
    rdfs:domain pdo:ActionItem;
    rdfs:range rdf:XMLLiteral .

pdo:hasEndTime a rdf:Property, owl:DatatypeProperty;
    rdfs:label "hadEndTime";
    rdfs:domain pdo:ActionItem;
    rdfs:range xsd:dateTime .

pdo:hasStartTime a rdf:Property, owl:DatatypeProperty;
    rdfs:label "hasStartTime";
    rdfs:domain pdo:ActionItem;
    rdfs:range xsd:dateTime .

pdo:hasStatus a rdf:Property, owl:DatatypeProperty;
    rdfs:label "hasStatus";
    rdfs:domain pdo:ActionItem;
    rdfs:range rdf:XMLLiteral .

pdo:contains a rdf:Property;
    rdfs:label "contains";
    rdfs:comment "The property which links an artefact (for example, an agenda item , an action item, a travle report, etc ) to the document in which it is mentioned.";
    rdfs:domain pdo:Document;
    rdfs:range pdo:Artefact .

pdo:isAssignedTo a rdf:Property;
    rdfs:label "isAssignedTo";
    rdfs:comment "This property links a pdo:ActionItem object to a foaf:Person object who is reponsible for the action item";
    rdfs:domain pdo:ActionItem;
    rdfs:range foaf:Person .

pdo:mentions a rdf:Property;
    rdfs:label "mentions";
    rdfs:comment "The property which links an artefact (for example, an agenda item , an action item, a travle report, etc ) to the document in which it is mentioned.";
    rdfs:domain
        pdo:Artefact,
        pdo:Comment,
        pdo:Document;
    rdfs:range rdf:Resource .
